moving all mem stuff to `SHOperator_Mem` class.

coq/SigmaHCOL/MemVecEq.v
@@ -42,441 +42,950 @@ Require Import ExtLib.Structures.Monoid.
 
 Require Import Coq.Lists.SetoidList.
 Require Import CoLoR.Util.List.ListUtil.
+Require Import CoLoR.Util.Nat.NatUtil.
 
 Import Monoid.
 
 Import VectorNotations.
 Open Scope vector_scope.
 
-Class SHOperator_MemVecEq
+Open Scope nat_scope.
+
+Class SHOperator_Mem
       {fm}
       {i o: nat}
-      (f: @SHOperator fm i o)
-      `{facts: SHOperator_Facts _ _ _ f}
+      (xop: @SHOperator fm i o)
+      `{facts: SHOperator_Facts fm _ _ xop}
   :=
     {
+      (* -- implementation on memory blocks -- *)
+      mem_op: mem_block -> option mem_block;
+      mem_op_proper: Proper ((=) ==> (=)) mem_op;
+      (* -- Structural properties for [mem_op] -- *)
+
+      (* sufficiently (values in right places, no info on empty
+         spaces) filled input memory block guarantees that `mem_op`
+         will not fail.  *)
+      mem_out_some: forall m,
+          (forall j (jc:j<i), in_index_set fm xop (mkFinNat jc) -> mem_in j m)
+          ->
+          is_Some (mem_op m);
+
+      (* Output memory block always have values in right places, and
+             does not have value in sparse positions *)
+      out_mem_fill_pattern: forall m0 m,
+          mem_op m0 ≡ Some m
+          ->
+          forall j (jc:j<o), out_index_set fm xop (mkFinNat jc) <-> mem_in j m;
+
+      (* Do not access memory outside of bounds *)
+      out_mem_oob: forall m0 m,
+          mem_op m0 ≡ Some m -> forall j (jc:j>=o), not (mem_in j m);
+
+      (* -- Semantics eqivalence -- *)
+
       mem_vec_preservation:
         forall x,
 
           (* Only for inputs which comply to `facts` *)
           (∀ (j : nat) (jc : (j < i)%nat),
-              in_index_set fm f (mkFinNat jc) → Is_Val (Vnth x jc))
+              in_index_set fm xop (mkFinNat jc) → Is_Val (Vnth x jc))
           ->
-          Some (svector_to_mem_block (op fm f x)) =
-          mem_op fm f (svector_to_mem_block x)
-      ;
+          Some (svector_to_mem_block (op fm xop x)) =
+          mem_op (svector_to_mem_block x);
     }.
 
 
 Section MemVecEq.
 
-  Section WithMonoid.
-    Variable fm:Monoid RthetaFlags.
-    Variable fml:@MonoidLaws RthetaFlags RthetaFlags_type fm.
+  (* !!!
+  (* Shinks family from [(S (S n))] to [(S n)], assuming [j] is below [(S n)] *)
+  Fact IUnion_mem_aux_shrink
+       {i o: nat}
+       (n : nat)
+       (j: nat) (jc: j<S n)
+       (op_family : SHOperatorFamily Monoid_RthetaFlags)
+       (m : NatMap CarrierA)
+    :
+      IUnion_mem_aux jc
+                     (get_family_mem_op Monoid_RthetaFlags
+                                        (shrink_op_family Monoid_RthetaFlags op_family))
+                     m
+                     ≡ IUnion_mem_aux
+                     (Nat.lt_lt_succ_r jc)
+                     (get_family_mem_op (i:=i) (o:=o) Monoid_RthetaFlags op_family) m.
+  Proof.
+    induction j.
+    -
+      unfold get_family_mem_op, shrink_op_family, mkFinNat.
+      simpl.
+      f_equiv; f_equiv; f_equiv.
+      apply le_unique.
+    -
+      simpl.
+      replace (get_family_mem_op Monoid_RthetaFlags
+                                 (shrink_op_family Monoid_RthetaFlags op_family) (S j) jc m)
+        with
+          (get_family_mem_op Monoid_RthetaFlags op_family (S j) (Nat.lt_lt_succ_r jc) m).
+      2:{
+        unfold get_family_mem_op, shrink_op_family, mkFinNat.
+        simpl.
+        f_equiv; f_equiv; f_equiv.
+        apply le_unique.
+      }
+      break_match; try reflexivity.
+      rewrite IHj.
+      replace (Nat.lt_lt_succ_r (Nat.lt_succ_l j (S n) jc)) with
+          (Nat.lt_succ_l j (S (S n)) (Nat.lt_lt_succ_r jc)) by apply le_unique.
+      reflexivity.
+  Qed.
+   *)
 
-    Global Instance compose_MemVecEq
+  Definition FinNatSet_to_natSet {n:nat} (f: FinNatSet n): Ensemble nat
+    := fun j => match lt_ge_dec j n with
+             | left jc => f (mkFinNat jc)
+             | in_right => False
+             end.
+
+  Lemma FinNatSet_to_natSet_Empty (f: FinNatSet 0):
+    FinNatSet_to_natSet f ≡ Empty_set _.
+  Proof.
+    apply Extensionality_Ensembles.
+    split; intros H P.
+    -
+      exfalso.
+      unfold FinNatSet_to_natSet in P.
+      unfold Ensembles.In in *.
+      break_match.
+      nat_lt_0_contradiction.
+      congruence.
+    -
+      contradict P.
+  Qed.
+
+  Lemma Disjoint_FinNat_to_nat {n:nat} (A B: FinNatSet n):
+    Disjoint _ A B ->
+    Disjoint nat (FinNatSet_to_natSet A) (FinNatSet_to_natSet B).
+  Proof.
+    intros D.
+    apply Disjoint_intro.
+    intros k C.
+    destruct D as [D].
+    destruct C as [k C1 C2].
+    unfold FinNatSet_to_natSet in *.
+    unfold Ensembles.In in *.
+    destruct (lt_ge_dec k n) as [kc | nkc].
+    -
+      specialize (D (mkFinNat kc)).
+      contradict D.
+      apply Intersection_intro.
+      + apply C1.
+      + apply C2.
+    -
+      tauto.
+  Qed.
+
+  Lemma mem_keys_set_to_out_index_set
+        (i o: nat)
+        {fm}
+        (xop: @SHOperator fm i o)
+        `{mop: SHOperator_Mem fm _ _ xop}
+        (m m0: mem_block)
+    :
+      (mem_op m0 ≡ Some m)
+      ->
+      FinNatSet_to_natSet (out_index_set fm xop) ≡ NE.mkEns (mem_keys_set m).
+  Proof.
+    intros H.
+    pose proof (out_mem_fill_pattern _ _ H) as H1.
+    pose proof (out_mem_oob _ _ H) as H2.
+    clear H.
+    unfold mem_in in *.
+    apply Extensionality_Ensembles.
+    unfold Same_set.
+    split.
+    -
+      unfold Ensembles.Included.
+      intros k H.
+      destruct (lt_ge_dec k o) as [kc | nkc].
+      +
+        clear H2.
+        specialize (H1 k kc).
+        apply mem_keys_set_In.
+        apply H1. clear H1.
+        unfold Ensembles.In in *.
+        generalize dependent (out_index_set fm xop).
+        intros s H.
+        unfold FinNatSet_to_natSet in H.
+        break_match_hyp; try contradiction.
+        replace l with kc in H by apply lt_unique.
+        apply H.
+      +
+        exfalso.
+        clear H1.
+        specialize (H2 k nkc).
+        (* H is false, as k is out of range *)
+        unfold Ensembles.In in H.
+        unfold FinNatSet_to_natSet in H.
+        break_match_hyp; try omega.
+    -
+      unfold Ensembles.Included.
+      intros k H.
+      unfold Ensembles.In in *.
+      destruct (lt_ge_dec k o) as [kc | nkc].
+      +
+        clear H2.
+        specialize (H1 k kc).
+        unfold FinNatSet_to_natSet.
+        break_match; try omega.
+        replace l with kc by apply lt_unique.
+        apply H1.
+        apply mem_keys_set_In.
+        apply H.
+      +
+        apply mem_keys_set_In in H.
+        specialize (H2 k nkc).
+        congruence.
+  Qed.
+
+  (*
+  Lemma IUnion_mem_aux_step_disjoint
+        (i o n : nat)
+        (j: nat) (jc: j < S (S n))
+        (k: nat) (kc: k < S (S n))
+        (jk: j<k)
+        (op_family: @SHOperatorFamily Monoid_RthetaFlags i o (S (S n)))
+        (op_family_facts: ∀ (j : nat) (jc : j < S (S n)),
+            @SHOperator_Facts Monoid_RthetaFlags i o
+                              (op_family (@mkFinNat (S (S n)) j jc)))
+
+        (compat : ∀ (m0 : nat) (mc : m0 < S (S n)) (n0 : nat) (nc : n0 < S (S n)),
+            m0 ≢ n0
+            → Disjoint (FinNat o)
+                       (@out_index_set Monoid_RthetaFlags i o (op_family (@mkFinNat (S (S n)) m0 mc)))
+                       (@out_index_set Monoid_RthetaFlags i o (op_family (@mkFinNat (S (S n)) n0 nc))))
+
+        (m m0 m1 : mem_block)
+
+        (H0: @get_family_mem_op Monoid_RthetaFlags i o (S (S n)) op_family
+                                k kc m
+                                ≡ @Some mem_block m0)
+        (H1:
+           @IUnion_mem_aux (S (S n))
+                           j jc
+                           (@get_family_mem_op
+                              Monoid_RthetaFlags i o
+                              (S (S n)) op_family) m
+                           ≡ @Some mem_block m1)
+    :
+      Disjoint nat
+               (NE.mkEns (mem_keys_set m0))
+               (NE.mkEns (mem_keys_set m1)).
+  Proof.
+    unfold get_family_mem_op in *.
+    revert m0 m1 k kc jk H0 H1.
+    induction j; intros.
+    -
+      assert(P: k <> 0) by auto.
+      assert(P1: k < S (S n)) by omega.
+      assert(P2: 0 < S (S n)) by lia.
+      specialize (compat k P1 0 P2 P).
+      clear P.
+      simpl in *.
+      apply Disjoint_FinNat_to_nat in compat.
+      rewrite
+        mem_keys_set_to_out_index_set
+        with (m:=m0) (m0:=m),
+             mem_keys_set_to_out_index_set
+        with (m:=m1) (m0:=m) in compat; auto.
+
+      rewrite <- H1; unfold mkFinNat;f_equiv; f_equiv; f_equiv; apply lt_unique.
+      rewrite <- H0; unfold mkFinNat; f_equiv; f_equiv;f_equiv; apply lt_unique.
+    -
+      simpl in *.
+      repeat break_match_hyp; try some_none.
+      apply (Disjoint_of_mem_merge H1).
+      +
+        assert(P: k ≢ S j) by lia.
+        specialize (compat k kc (S j) jc P).
+        simpl in compat.
+        erewrite <- 2!mem_keys_set_to_out_index_set.
+        apply Disjoint_FinNat_to_nat.
+        eapply compat.
+        eauto.
+        eauto.
+        eauto.
+        eauto.
+      +
+        unshelve eapply IHj ; try auto; try omega.
+        replace (dec_not_not _ _ _) with (Nat.lt_succ_l j (S (S n)) jc)
+          by apply lt_unique.
+        apply Heqo1.
+  Qed.
+
+  (* Shinks family from `(S (S n))` to `(S n)`, assuming `j` is below `(S n)` *)
+  Fact IReduction_mem_aux_shrink
+       {i o: nat}
+       (n : nat)
+       (j: nat) (jc: j<S n)
+       (dot : CarrierA → CarrierA → CarrierA)
+       (op_family : SHOperatorFamily Monoid_RthetaSafeFlags)
+       (m : NatMap CarrierA)
+    :
+      IReduction_mem_aux jc dot
+                         (get_family_mem_op Monoid_RthetaSafeFlags
+                                            (shrink_op_family Monoid_RthetaSafeFlags op_family))
+                         m
+                         ≡ IReduction_mem_aux
+                         (Nat.lt_lt_succ_r jc)
+                         dot
+                         (get_family_mem_op (i:=i) (o:=o) Monoid_RthetaSafeFlags op_family) m.
+  Proof.
+    induction j.
+    -
+      unfold get_family_mem_op, shrink_op_family, mkFinNat.
+      simpl.
+      f_equiv; f_equiv; f_equiv.
+      apply le_unique.
+    -
+      simpl.
+      replace (get_family_mem_op Monoid_RthetaSafeFlags
+                                 (shrink_op_family Monoid_RthetaSafeFlags op_family) (S j) jc m)
+        with
+          (get_family_mem_op Monoid_RthetaSafeFlags op_family (S j) (Nat.lt_lt_succ_r jc) m).
+      2:{
+        unfold get_family_mem_op, shrink_op_family, mkFinNat.
+        simpl.
+        f_equiv; f_equiv; f_equiv.
+        apply le_unique.
+      }
+      break_match; try reflexivity.
+      rewrite IHj.
+      replace (Nat.lt_lt_succ_r (Nat.lt_succ_l j (S n) jc)) with
+          (Nat.lt_succ_l j (S (S n)) (Nat.lt_lt_succ_r jc)) by apply le_unique.
+      reflexivity.
+  Qed.
+   *)
+
+  Section WithMonoid.
+
+    Variable fm: Monoid RthetaFlags.
+    Variable fml: @MonoidLaws RthetaFlags RthetaFlags_type fm.
+
+    Global Instance compose_Mem
            {i1 o2 o3}
            (op1: @SHOperator fm o2 o3)
            (op2: @SHOperator fm i1 o2)
            (compat: Included _ (in_index_set fm op1) (out_index_set fm op2))
-           `{Meq1: SHOperator_MemVecEq fm o2 o3 op1}
-           `{Meq2: SHOperator_MemVecEq fm i1 o2 op2}
-      : SHOperator_MemVecEq
-          (facts:=SHCompose_Facts fm  op1 op2 compat)
+           `{Meq1: SHOperator_Mem fm o2 o3 op1}
+           `{Meq2: SHOperator_Mem fm i1 o2 op2}
+      : SHOperator_Mem
+          (facts:=SHCompose_Facts fm op1 op2 compat)
           (SHCompose fm op1 op2).
     Proof.
-      split.
-      intros x G.
-      simpl.
-      unfold option_compose, compose.
-      simpl in G.
+      unshelve esplit.
+      -
+        exact (option_compose (mem_op (xop:=op1))
+                              (mem_op (xop:=op2))
+              ).
+      -
+        apply option_compose_proper; [ apply Meq1 | apply Meq2].
+      -
+        (* mem_out_some *)
+        intros m H.
+        unfold is_Some, option_compose in *.
+        simpl in *.
+        unfold option_compose.
+        repeat break_match; try some_none; try auto.
+        +
+          contradict Heqo.
+          apply is_Some_ne_None.
+          apply mem_out_some.
+          pose proof (out_mem_fill_pattern m m0 Heqo0) as P.
+          intros j jc H0.
+          specialize (P j jc).
+          apply P.
+          apply compat.
+          apply H0.
+        +
+          clear Heqo.
+          pose proof (@mem_out_some _ _ _ _ _ _ _ H) as C.
+          unfold is_Some in C.
+          break_match; [ some_none | tauto].
+      -
+        (* out_mem_fill_pattern *)
+        intros m0 m H.
+        split.
+        +
+          simpl in *.
+          unfold option_compose in H.
+          break_match_hyp; try some_none.
+          pose proof (out_mem_fill_pattern  m1 m H) as P1.
+          apply P1; auto.
+        +
+          simpl in *.
+          unfold option_compose in H.
+          break_match_hyp; try some_none.
+          pose proof (out_mem_fill_pattern m1 m H) as P2.
+          apply P2; auto.
+      -
+        (* mem_out_oob *)
+        intros m0 m H.
+        unfold option_compose in H.
+        break_match_hyp; try some_none.
+        pose proof (out_mem_oob  m1 m H) as P2.
+        apply P2; auto.
+      -
+        (* mem_vec_preservation *)
+        intros x G.
+        unfold option_compose, compose.
+        simpl in G.
 
-      pose proof (@mem_out_some fm _ _ op2 _ (svector_to_mem_block x) ) as Rm.
-      assert(G0: (∀ (j : nat) (jc : (j < i1)%nat), in_index_set fm op2 (mkFinNat jc)
-                                         → mem_in j (svector_to_mem_block x))).
-      {
-        intros j jc H.
-        apply svector_to_mem_block_In with (jc0:=jc).
-        apply G,H.
-      }
-      specialize (Rm G0).
-      apply is_Some_equiv_def in Rm.
-      destruct Rm as [m2 Rm].
-      break_match; try some_none.
-      clear Rm m2.
-      pose proof (mem_op_proper _ op1) as P.
-      setoid_replace m with (svector_to_mem_block (op fm op2 x)).
-      apply Meq1.
-      {
-        intros j jc H.
-        apply facts0. (* out_as_range *)
-        apply G.
-        apply compat, H.
-      }
+        pose proof (@mem_out_some fm _ _ op2 _ Meq2 (svector_to_mem_block x) ) as Rm.
+        assert(G0: (∀ (j : nat) (jc : (j < i1)%nat), in_index_set fm op2 (mkFinNat jc)
+                                                 → mem_in j (svector_to_mem_block x))).
+        {
+          intros j jc H.
+          apply svector_to_mem_block_In with (jc0:=jc).
+          apply G,H.
+        }
+        specialize (Rm G0).
+        apply is_Some_equiv_def in Rm.
+        destruct Rm as [m2 Rm].
+        break_match; try some_none.
+        clear Rm m2.
+        pose proof (mem_op_proper (xop:=op1)) as P.
+        setoid_replace m with (svector_to_mem_block (op fm op2 x)).
+        apply Meq1.
+        {
+          intros j jc H.
+          apply facts0. (* out_as_range *)
+          apply G.
+          apply compat, H.
+        }
 
-      apply Some_inj_equiv.
-      rewrite <- Heqo.
-      symmetry.
-      apply Meq2, G.
+        apply Some_inj_equiv.
+        rewrite <- Heqo.
+        symmetry.
+        apply Meq2, G.
     Qed.
 
-    Global Instance liftM_MemVecEq
+    Global Instance liftM_Mem
            {i o}
            (hop: avector i -> avector o)
            `{HOP: HOperator i o hop}
-      : SHOperator_MemVecEq (liftM_HOperator fm hop).
+      : SHOperator_Mem (liftM_HOperator fm hop).
     Proof.
-      assert (facts: SHOperator_Facts fm (liftM_HOperator fm hop)) by
-          typeclasses eauto.
-      split.
-      intros x G.
-      simpl.
-      unfold mem_op_of_hop.
-      unfold liftM_HOperator', avector_to_mem_block, svector_to_mem_block, compose in *.
-
-      svector_to_mem_block_to_spec m0 H0 I0 O0.
-      svector_to_mem_block_to_spec m1 H1 I1 O1.
-      break_match.
+      unshelve esplit.
       -
-        f_equiv.
-        avector_to_mem_block_to_spec m2 H2 O2.
-        simpl in *.
-        unfold equiv, mem_block_Equiv, mem_block_equiv, NM.Equal.
-        intros k.
-        destruct (NatUtil.lt_ge_dec k o) as [H | H].
-        +
-          clear O0 O1 O2.
-          specialize (H0 k H).
-          specialize (H2 k H).
-          assert(V: Is_Val (Vnth (sparsify fm (hop (densify fm x))) H)).
-          {
-            destruct facts.
-            apply out_as_range.
-            intros j jc H9.
-            apply G.
-            apply Full_intro.
-            apply Full_intro.
-          }
-          rewrite NP.F.find_mapsto_iff in H0.
-          apply H0 in V.
-          unfold mem_lookup in *.
+        exact (mem_op_of_hop hop).
+      -
+        typeclasses eauto.
+      -
+        (* mem_out_some *)
+        intros m H.
+        apply mem_out_some_mem_op_of_hop, H.
+      -
+        simpl.
+        intros m0 m H.
+        apply (out_mem_fill_pattern_mem_op_of_hop H).
+      -
+        simpl.
+        intros m0 m H.
+        apply (out_mem_fill_pattern_mem_op_of_hop H).
+      -
+        (* mem_vec_preservation *)
+        assert (facts: SHOperator_Facts fm (liftM_HOperator fm hop)) by
+            typeclasses eauto.
 
-          rewrite H2, V. clear H2 V.
-          unfold sparsify.
-          rewrite Vnth_map.
-          rewrite evalWriter_mkValue.
-          unfold densify.
-          unfold mem_block_to_avector, mem_lookup in Heqo0.
-          apply vsequence_Vbuild_eq_Some in Heqo0.
+        intros x G.
+        simpl.
+        unfold mem_op_of_hop.
+        unfold liftM_HOperator', avector_to_mem_block, svector_to_mem_block, compose in *.
+
+        svector_to_mem_block_to_spec m0 H0 I0 O0.
+        svector_to_mem_block_to_spec m1 H1 I1 O1.
+        break_match.
+        +
           f_equiv.
-          apply Vnth_arg_equiv.
-          f_equiv.
-          vec_index_equiv j jc.
-          assert(V0: Is_Val (Vnth x jc)).
-          {
-            apply G.
-            apply Full_intro.
-          }
-          apply H1 in V0.
-          rewrite NP.F.find_mapsto_iff in V0.
-          rewrite Vnth_map.
-          apply Vnth_arg_eq with (ip:=jc) in Heqo0.
-          rewrite Vbuild_nth in Heqo0.
-          rewrite Vnth_map in Heqo0.
-          rewrite V0 in Heqo0.
-          inversion Heqo0.
-          reflexivity.
-        +
-          rewrite O0, O2 by apply H.
-          reflexivity.
-      -
-        simpl in *.
-        unfold mem_block_to_avector in Heqo0.
-        apply vsequence_Vbuild_eq_None in Heqo0.
-        destruct Heqo0 as [j [jc Heqo0]].
-        assert(V0: Is_Val (Vnth x jc)).
-        {
-          apply G.
-          apply Full_intro.
-        }
-        apply H1 in V0. clear H1.
-        apply NP.F.find_mapsto_iff in V0.
-        unfold mem_lookup in Heqo0.
-        congruence.
-    Qed.
-
-    Global Instance eUnion_MemVecEq
-           {o b:nat}
-           (bc: b < o)
-           (z: CarrierA)
-      : SHOperator_MemVecEq (eUnion fm bc z).
-    Proof.
-      assert (facts: SHOperator_Facts fm (eUnion fm bc z)) by
-          typeclasses eauto.
-      split.
-      intros x G.
-      simpl.
-      unfold eUnion_mem, map_mem_block_elt.
-
-      unfold svector_to_mem_block.
-      svector_to_mem_block_to_spec m0 H0 I0 O0.
-      svector_to_mem_block_to_spec m1 H1 I1 O1.
-
-      break_match; unfold mem_lookup in *; simpl in *.
-      -
-        f_equiv.
-        unfold mem_add, mem_empty.
-        assert(Vb: Is_Val (Vnth (eUnion' bc z x) bc)).
-        {
-          destruct facts.
-          apply out_as_range.
-          -
-            intros j jc H.
-            apply G.
-            auto.
-          -
-            simpl.
-            reflexivity.
-        }
-        unfold equiv, mem_block_Equiv, mem_block_equiv, NM.Equal.
-        intros k.
-        (* MapsTo *)
-        destruct (NatUtil.lt_ge_dec k o) as [kc | kc].
-        +
-          (* k<o, which is normal *)
-          clear O0 O1.
-          destruct (eq_nat_dec b k) as [E | NE].
+          avector_to_mem_block_to_spec m2 H2 O2.
+          simpl in *.
+          unfold equiv, mem_block_Equiv, mem_block_equiv, NM.Equal.
+          intros k.
+          destruct (NatUtil.lt_ge_dec k o) as [H | H].
           *
-            (* b = k *)
-            subst k.
-            specialize (H0 b bc).
-            specialize (I0 b bc).
-            apply H0 in Vb; clear H0.
-            apply NM.find_1 in Vb.
-            rewrite_clear Vb.
-            rewrite NP.F.add_eq_o by reflexivity.
+            clear O0 O1 O2.
+            specialize (H0 k H).
+            specialize (H2 k H).
+            assert(V: Is_Val (Vnth (sparsify fm (hop (densify fm x))) H)).
+            {
+              destruct facts.
+              apply out_as_range.
+              intros j jc H9.
+              apply G.
+              apply Full_intro.
+              apply Full_intro.
+            }
+            rewrite NP.F.find_mapsto_iff in H0.
+            apply H0 in V.
+            unfold mem_lookup in *.
+
+            rewrite H2, V. clear H2 V.
+            unfold sparsify.
+            rewrite Vnth_map.
+            rewrite evalWriter_mkValue.
+            unfold densify.
+            unfold mem_block_to_avector, mem_lookup in Heqo0.
+            apply vsequence_Vbuild_eq_Some in Heqo0.
             f_equiv.
-            unfold eUnion'.
-            rewrite Vbuild_nth.
-            dep_destruct (Nat.eq_dec b b); try congruence.
-
-            specialize (H1 0 (lt_0_Sn 0)).
-            specialize (I1 0 (lt_0_Sn 0)).
-            rewrite NP.F.find_mapsto_iff in H1.
-
-            assert(V0: Is_Val (Vnth x (Nat.lt_0_succ 0))).
+            apply Vnth_arg_equiv.
+            f_equiv.
+            vec_index_equiv j jc.
+            assert(V0: Is_Val (Vnth x jc)).
             {
               apply G.
               apply Full_intro.
             }
             apply H1 in V0.
-            unfold zero in V0.
+            rewrite NP.F.find_mapsto_iff in V0.
+            rewrite Vnth_map.
+            apply Vnth_arg_eq with (ip:=jc) in Heqo0.
+            rewrite Vbuild_nth in Heqo0.
+            rewrite Vnth_map in Heqo0.
             rewrite V0 in Heqo0.
-            some_inv.
-            rewrite Vnth_0.
+            inversion Heqo0.
             reflexivity.
           *
-            (* k<o, which is normal *)
-            (* b!=k *)
-            rewrite NP.F.add_neq_o by apply NE.
-            rewrite NP.F.empty_o.
-
-            assert(Vk: Is_Struct (Vnth (eUnion' bc z x) kc)).
-            {
-              destruct facts.
-              apply no_vals_at_sparse.
-              auto.
-            }
-            clear H1 I1 m1 Heqo0.
-
-            apply NP.F.not_find_in_iff.
-            unfold not.
-            intros H.
-
-            specialize (I0 k kc).
-            apply I0 in H.
-            crush.
+            rewrite O0, O2 by apply H.
+            reflexivity.
         +
-          (* k>=o, oob case *)
-          specialize (O0 k kc).
-          rewrite_clear O0.
-          rewrite NP.F.add_neq_o by (unfold lt, nat_lt in bc;omega).
-          rewrite NP.F.empty_o.
-          reflexivity.
-      -
-        exfalso.
-        assert(V:Is_Val (Vnth x (Nat.lt_0_succ 0))).
-        {
-          apply G.
-          apply Full_intro.
-        }
-        specialize (H1 0 (lt_0_Sn 0)).
-        apply H1 in V; clear H1.
-        apply NP.F.find_mapsto_iff in V.
-        unfold zero in *.
-        congruence.
+          simpl in *.
+          unfold mem_block_to_avector in Heqo0.
+          apply vsequence_Vbuild_eq_None in Heqo0.
+          destruct Heqo0 as [j [jc Heqo0]].
+          assert(V0: Is_Val (Vnth x jc)).
+          {
+            apply G.
+            apply Full_intro.
+          }
+          apply H1 in V0. clear H1.
+          apply NP.F.find_mapsto_iff in V0.
+          unfold mem_lookup in Heqo0.
+          congruence.
     Qed.
 
-    Global Instance eT_MemVecEq
+    Global Instance eUnion_Mem
            {o b:nat}
            (bc: b < o)
-      : SHOperator_MemVecEq (eT fm bc).
+           (z: CarrierA)
+      : SHOperator_Mem (eUnion fm bc z).
     Proof.
-      assert (facts: SHOperator_Facts fm (eT fm bc)) by
-          typeclasses eauto.
-      split.
-      intros x G.
-      simpl.
 
-      unfold eT_mem , map_mem_block_elt.
-      unfold svector_to_mem_block.
-      svector_to_mem_block_to_spec m0 H0 I0 O0.
-      svector_to_mem_block_to_spec m1 H1 I1 O1.
-      Opaque Vnth.
-      simpl in *.
-
-      break_match.
+      unshelve esplit.
       -
-        f_equiv.
-        unfold equiv, mem_block_Equiv, mem_block_equiv, NM.Equal.
-        intros k.
-        destruct (NatUtil.lt_ge_dec k 1) as [kc | kc].
+        apply (eUnion_mem b).
+      -
+        typeclasses eauto.
+      -
+        (* mem_out_some *)
+        intros m H.
+        unfold is_Some, eUnion, eUnion_mem, map_mem_block_elt, mem_lookup. simpl.
+        repeat break_match; try some_none; try tauto.
+        clear Heqo0. rename Heqo1 into M.
+        simpl in *.
+        assert(P: Full_set (FinNat 1) (mkFinNat Nat.lt_0_1)) by apply Full_intro.
+        apply H in P.
+        unfold mem_lookup, mem_in in *.
+        apply NP.F.not_find_in_iff in M.
+        congruence.
+      -
+        (* out_mem_fill_pattern *)
+        intros m0 m H.
+        split.
         +
-          clear O0 O1 I0 I1.
+          simpl in *.
+          unfold eUnion_mem, map_mem_block_elt, mem_lookup, mem_in, mem_add, mem_empty in *.
+          break_match_hyp; try some_none.
+          some_inv.
+          subst m.
+          intros O.
+          destruct (eq_nat_dec j b).
+          --
+            apply NP.F.in_find_iff.
+            rewrite NP.F.add_eq_o; auto.
+            some_none.
+          --
+            unfold FinNatSet.singleton, mkFinNat in O.
+            simpl in O.
+            congruence.
+        +
+          simpl in *.
+          unfold eUnion_mem, map_mem_block_elt, mem_lookup, mem_in, mem_add, mem_empty in *.
+          break_match_hyp; try some_none.
+          some_inv.
+          subst m.
+          intros I.
+          unfold FinNatSet.singleton, mkFinNat.
+          destruct (eq_nat_dec j b); auto.
+          exfalso.
+          apply NP.F.in_find_iff in I.
+          rewrite NP.F.add_neq_o in I ; auto.
+      -
+        intros m0 m H j jc C.
+        simpl in H.
+        unfold eUnion_mem, map_mem_block_elt, mem_lookup, mem_in in *. simpl in *.
+        break_match; try some_none.
+        some_inv.
+        subst m.
+        unfold mem_add, mem_empty in C.
+        destruct (eq_nat_dec j b); try omega.
+        apply NP.F.in_find_iff in C.
+        rewrite NP.F.add_neq_o in C; auto.
+      -
+        assert (facts: SHOperator_Facts fm (eUnion fm bc z)) by
+            typeclasses eauto.
+        intros x G.
+        simpl.
+        unfold eUnion_mem, map_mem_block_elt.
 
+        unfold svector_to_mem_block.
+        svector_to_mem_block_to_spec m0 H0 I0 O0.
+        svector_to_mem_block_to_spec m1 H1 I1 O1.
+
+        break_match; unfold mem_lookup in *; simpl in *.
+        +
+          f_equiv.
+          unfold mem_add, mem_empty.
+          assert(Vb: Is_Val (Vnth (eUnion' bc z x) bc)).
+          {
+            destruct facts.
+            apply out_as_range.
+            -
+              intros j jc H.
+              apply G.
+              auto.
+            -
+              simpl.
+              reflexivity.
+          }
+          unfold equiv, mem_block_Equiv, mem_block_equiv, NM.Equal.
+          intros k.
+          (* MapsTo *)
+          destruct (NatUtil.lt_ge_dec k o) as [kc | kc].
+          *
+            (* k<o, which is normal *)
+            clear O0 O1.
+            destruct (eq_nat_dec b k) as [E | NE].
+            --
+              (* b = k *)
+              subst k.
+              specialize (H0 b bc).
+              specialize (I0 b bc).
+              apply H0 in Vb; clear H0.
+              apply NM.find_1 in Vb.
+              rewrite_clear Vb.
+              rewrite NP.F.add_eq_o by reflexivity.
+              f_equiv.
+              unfold eUnion'.
+              rewrite Vbuild_nth.
+              dep_destruct (Nat.eq_dec b b); try congruence.
+
+              specialize (H1 0 (lt_0_Sn 0)).
+              specialize (I1 0 (lt_0_Sn 0)).
+              rewrite NP.F.find_mapsto_iff in H1.
+
+              assert(V0: Is_Val (Vnth x (Nat.lt_0_succ 0))).
+              {
+                apply G.
+                apply Full_intro.
+              }
+              apply H1 in V0.
+              unfold zero in V0.
+              rewrite V0 in Heqo0.
+              some_inv.
+              rewrite Vnth_0.
+              reflexivity.
+            --
+              (* k<o, which is normal *)
+              (* b!=k *)
+              rewrite NP.F.add_neq_o by apply NE.
+              rewrite NP.F.empty_o.
+
+              assert(Vk: Is_Struct (Vnth (eUnion' bc z x) kc)).
+              {
+                destruct facts.
+                apply no_vals_at_sparse.
+                auto.
+              }
+              clear H1 I1 m1 Heqo0.
+
+              apply NP.F.not_find_in_iff.
+              unfold not.
+              intros H.
+
+              specialize (I0 k kc).
+              apply I0 in H.
+              crush.
+          *
+            (* k>=o, oob case *)
+            specialize (O0 k kc).
+            rewrite_clear O0.
+            rewrite NP.F.add_neq_o by (unfold lt, nat_lt in bc;omega).
+            rewrite NP.F.empty_o.
+            reflexivity.
+        +
+          exfalso.
+          assert(V:Is_Val (Vnth x (Nat.lt_0_succ 0))).
+          {
+            apply G.
+            apply Full_intro.
+          }
+          specialize (H1 0 (lt_0_Sn 0)).
+          apply H1 in V; clear H1.
+          apply NP.F.find_mapsto_iff in V.
+          unfold zero in *.
+          congruence.
+    Qed.
+
+    Global Instance eT_Mem
+           {o b:nat}
+           (bc: b < o)
+      : SHOperator_Mem (eT fm bc).
+    Proof.
+      unshelve esplit.
+      -
+        apply (eT_mem b).
+      -
+        typeclasses eauto.
+      -
+        (* mem_out_some *)
+        intros v H.
+        unfold is_Some, eT, eT_mem, map_mem_block_elt, mem_lookup. simpl.
+        repeat break_match; try some_none; try tauto.
+        clear Heqo0. rename Heqo1 into M.
+        simpl in *.
+        assert(P: FinNatSet.singleton b (mkFinNat bc)).
+        {
+          unfold FinNatSet.singleton, mkFinNat.
+          auto.
+        }
+        apply H in P.
+        unfold mem_lookup, mem_in in *.
+        apply NP.F.not_find_in_iff in M.
+        congruence.
+      -
+        (* out_mem_fill_pattern *)
+        intros m0 m H.
+        simpl in *.
+        unfold eT_mem, map_mem_block_elt, mem_lookup, mem_in in *.
+        destruct j; try omega.
+        split.
+        +
+          intros F.
+          break_match_hyp; try some_none.
+          some_inv.
+          subst m.
+          unfold mem_add, mem_empty.
+          apply NP.F.in_find_iff.
+          rewrite NP.F.add_eq_o.
+          some_none.
+          reflexivity.
+        +
+          intros I.
+          apply Full_intro.
+      -
+        intros m0 m H.
+        simpl in *.
+        unfold eT_mem, map_mem_block_elt, mem_lookup, mem_in in *.
+
+        intros j jc.
+        unfold not.
+        intros C.
+        break_match_hyp; try some_none.
+        some_inv.
+        subst m.
+        unfold mem_add, mem_empty in *.
+        destruct (eq_nat_dec j 0) as [z | nz].
+        +
+          lia.
+        +
+          apply NP.F.add_neq_in_iff in C.
+          apply NP.F.empty_in_iff in C.
+          tauto.
+          auto.
+      -
+        assert (facts: SHOperator_Facts fm (eT fm bc)) by
+            typeclasses eauto.
+        intros x G.
+        simpl.
+
+        unfold eT_mem , map_mem_block_elt.
+        unfold svector_to_mem_block.
+        svector_to_mem_block_to_spec m0 H0 I0 O0.
+        svector_to_mem_block_to_spec m1 H1 I1 O1.
+        Opaque Vnth.
+        simpl in *.
+        break_match.
+        +
+          f_equiv.
+          unfold equiv, mem_block_Equiv, mem_block_equiv, NM.Equal.
+          intros k.
+          destruct (NatUtil.lt_ge_dec k 1) as [kc | kc].
+          *
+            clear O0 O1 I0 I1.
+
+            assert (Is_Val (Vnth x bc)) as V.
+            {
+              apply G.
+              reflexivity.
+            }
+            apply H1 in V. clear H1.
+            apply NM.find_1 in V.
+            unfold mem_lookup in Heqo0.
+            rewrite Heqo0 in V. clear Heqo0 m1.
+            some_inv. clear c H1.
+
+            assert(Is_Val (Vnth (eT' bc x) (lt_0_Sn O))) as V0.
+            {
+              unfold eT'.
+              rewrite Vnth_0.
+              simpl.
+              apply G.
+              reflexivity.
+            }
+            rewrite H0 in V0. clear H0.
+            apply NM.find_1 in V0.
+            rewrite NP.F.add_eq_o by omega.
+            destruct k.
+            --
+              rewrite V0.
+              f_equiv.
+            --
+              omega.
+          *
+            unfold mem_lookup in *.
+            rewrite O0 by apply kc.
+            rewrite NP.F.add_neq_o by omega.
+            rewrite NP.F.empty_o.
+            reflexivity.
+        +
           assert (Is_Val (Vnth x bc)) as V.
           {
             apply G.
             reflexivity.
           }
-          apply H1 in V. clear H1.
+          apply H1 in V.
           apply NM.find_1 in V.
           unfold mem_lookup in Heqo0.
-          rewrite Heqo0 in V. clear Heqo0 m1.
-          some_inv. clear c H1.
-
-          assert(Is_Val (Vnth (eT' bc x) (lt_0_Sn O))) as V0.
-          {
-            unfold eT'.
-            rewrite Vnth_0.
-            simpl.
-            apply G.
-            reflexivity.
-          }
-          rewrite H0 in V0. clear H0.
-          apply NM.find_1 in V0.
-          rewrite NP.F.add_eq_o by omega.
-          destruct k.
-          *
-            rewrite V0.
-            f_equiv.
-          *
-            omega.
-        +
-          unfold mem_lookup in *.
-          rewrite O0 by apply kc.
-          rewrite NP.F.add_neq_o by omega.
-          rewrite NP.F.empty_o.
-          reflexivity.
-      -
-        assert (Is_Val (Vnth x bc)) as V.
-        {
-          apply G.
-          reflexivity.
-        }
-        apply H1 in V.
-        apply NM.find_1 in V.
-        unfold mem_lookup in Heqo0.
-        congruence.
+          congruence.
     Qed.
 
-    Global Instance SHPointwise_MemVecEq
+    Global Instance SHPointwise_Mem
            {n: nat}
            (f: FinNat n -> CarrierA -> CarrierA)
            `{pF: !Proper ((=) ==> (=) ==> (=)) f}
-      : SHOperator_MemVecEq (SHPointwise fm f).
+      : SHOperator_Mem (SHPointwise fm f).
     Proof.
-      assert (facts: SHOperator_Facts fm (SHPointwise fm f)) by
-          typeclasses eauto.
+      unshelve esplit.
+      -
+        apply (mem_op_of_hop (HPointwise f)).
+      -
+        typeclasses eauto.
+      -
+        (* mem_out_some *)
+        intros v H.
+        apply mem_out_some_mem_op_of_hop, H.
+      -
+        intros m0 m H.
+        apply (out_mem_fill_pattern_mem_op_of_hop H).
+      -
+        intros m0 m H.
+        apply (out_mem_fill_pattern_mem_op_of_hop H).
+      -
+        assert (facts: SHOperator_Facts fm (SHPointwise fm f)) by
+            typeclasses eauto.
 
-      split.
-      intros x G.
-      simpl.
+        intros x G.
+        simpl.
 
-      pose proof (@mem_out_some _ _ _ _ facts (svector_to_mem_block x)) as M.
-      apply is_Some_equiv_def in M.
-      destruct M as [y M].
-      rewrite M.
-      f_equiv.
-      unfold equiv, mem_block_Equiv, mem_block_equiv, NM.Equal.
-      intros k.
+        assert((∀ (j : nat) (jc : j < n), in_index_set fm
+                                                     (SHPointwise fm f)
+                                                     (mkFinNat jc) →
+                                        mem_in j (svector_to_mem_block x))
+               → is_Some (mem_op_of_hop (HPointwise f) (svector_to_mem_block x))) as M by apply mem_out_some_mem_op_of_hop.
+        apply is_Some_equiv_def in M.
+        destruct M as [y M].
+        rewrite M.
+        f_equiv.
+        unfold equiv, mem_block_Equiv, mem_block_equiv, NM.Equal.
+        intros k.
 
-      unfold svector_to_mem_block in *.
-      svector_to_mem_block_to_spec m0 H0 I0 O0.
-      svector_to_mem_block_to_spec m1 H1 I1 O1.
-      simpl in *.
+        unfold svector_to_mem_block in *.
+        svector_to_mem_block_to_spec m0 H0 I0 O0.
+        svector_to_mem_block_to_spec m1 H1 I1 O1.
+        simpl in *.
 
-      unfold mem_op_of_hop in M.
-      break_match_hyp; try some_none.
-      some_inv.
-      rewrite <- M. clear M.
+        unfold mem_op_of_hop in M.
+        break_match_hyp; try some_none.
+        some_inv.
+        rewrite <- M. clear M.
 
-      unfold avector_to_mem_block.
-      avector_to_mem_block_to_spec m2 H2 O2.
-      unfold mem_lookup in *. simpl in *.
+        unfold avector_to_mem_block.
+        avector_to_mem_block_to_spec m2 H2 O2.
+        unfold mem_lookup in *. simpl in *.
 
-      destruct (NatUtil.lt_ge_dec k n) as [kc | kc].
-      +
-        (* k<n, which is normal *)
-        clear O0 O1 O2.
-        specialize (H0 k kc). specialize (I0 k kc).
-        specialize (H1 k kc). specialize (I1 k kc).
-        assert(V0: Is_Val (Vnth x kc)).
-        {
-          apply G.
-          apply Full_intro.
-        }
+        destruct (NatUtil.lt_ge_dec k n) as [kc | kc].
+        +
+          (* k<n, which is normal *)
+          clear O0 O1 O2.
+          specialize (H0 k kc). specialize (I0 k kc).
+          specialize (H1 k kc). specialize (I1 k kc).
+          assert(V0: Is_Val (Vnth x kc)).
+          {
+            apply G.
+            apply Full_intro.
+          }
 
-        assert(V: Is_Val (Vnth (SHPointwise' f x) kc)).
-        {
+          assert(V: Is_Val (Vnth (SHPointwise' f x) kc)).
+          {
+            unfold SHPointwise'.
+            rewrite Vbuild_nth.
+            apply Is_Val_liftM.
+            apply V0.
+          }
+
+          rewrite H0 in V.
+          apply NM.find_1 in V.
+          rewrite V.
+
           unfold SHPointwise'.
           rewrite Vbuild_nth.
-          apply Is_Val_liftM.
-          apply V0.
-        }
+          rewrite H2 with (ip:=kc).
+          rewrite HPointwise_nth.
+          rewrite evalWriter_Rtheta_liftM.
+          f_equiv.
+          f_equiv.
 
-        rewrite H0 in V.
-        apply NM.find_1 in V.
-        rewrite V.
+          unfold mem_block_to_avector in Heqo.
+          apply vsequence_Vbuild_eq_Some in Heqo.
+          apply Vnth_arg_eq with (ip:=kc) in Heqo.
+          rewrite Vbuild_nth in Heqo.
+          rewrite Vnth_map in Heqo.
+          unfold mem_lookup in Heqo.
 
-        unfold SHPointwise'.
-        rewrite Vbuild_nth.
-        rewrite H2 with (ip:=kc).
-        rewrite HPointwise_nth.
-        rewrite evalWriter_Rtheta_liftM.
-        f_equiv.
-        f_equiv.
-
-        unfold mem_block_to_avector in Heqo.
-        apply vsequence_Vbuild_eq_Some in Heqo.
-        apply Vnth_arg_eq with (ip:=kc) in Heqo.
-        rewrite Vbuild_nth in Heqo.
-        rewrite Vnth_map in Heqo.
-        unfold mem_lookup in Heqo.
-
-        apply H1 in V0.
-        apply NM.find_1 in V0.
-        rewrite Heqo in V0.
-        some_inv.
-        reflexivity.
-      +
-        rewrite O0 by apply kc.
-        rewrite O2 by apply kc.
-        reflexivity.
-      +
-        intros j jc HH.
-        apply svector_to_mem_block_In with (jc0:=jc).
-        apply G,HH.
+          apply H1 in V0.
+          apply NM.find_1 in V0.
+          rewrite Heqo in V0.
+          some_inv.
+          reflexivity.
+        +
+          rewrite O0 by apply kc.
+          rewrite O2 by apply kc.
+          reflexivity.
+        +
+          intros j jc HH.
+          apply svector_to_mem_block_In with (jc0:=jc).
+          apply G,HH.
     Qed.
 
   End WithMonoid.
@@ -516,122 +1025,140 @@ Section MemVecEq.
       destruct H.
       + apply H.
       + exfalso.
-        unfold In in H.
+        unfold Ensembles.In in H.
         destruct H.
         congruence.
   Qed.
 
   Section MonoidSpecific.
 
-    Global Instance SHBinOp_RthetaSafe_MemVecEq
+    Global Instance SHBinOp_RthetaSafe_Mem
            {o}
            (f: {n:nat|n<o} -> CarrierA -> CarrierA -> CarrierA)
            `{pF: !Proper ((=) ==> (=) ==> (=) ==> (=)) f}
-    : SHOperator_MemVecEq (@SHBinOp Monoid_RthetaSafeFlags o f pF).
+    : SHOperator_Mem (@SHBinOp Monoid_RthetaSafeFlags o f pF).
     Proof.
-      assert (facts: SHOperator_Facts _ (SHBinOp Monoid_RthetaSafeFlags f)) by
-          typeclasses eauto.
+      unshelve esplit.
+      -
+        apply (mem_op_of_hop (HBinOp f)).
+      -
+        typeclasses eauto.
+      -
+        intros v H.
+        apply mem_out_some_mem_op_of_hop, H.
+      -
+        intros m0 m H.
+        apply (out_mem_fill_pattern_mem_op_of_hop H).
+      -
+        intros m0 m H.
+        apply (out_mem_fill_pattern_mem_op_of_hop H).
+      -
+        assert (facts: SHOperator_Facts _ (SHBinOp Monoid_RthetaSafeFlags f)) by
+            typeclasses eauto.
 
-      split.
-      intros x G.
-      simpl.
+        intros x G.
+        simpl.
 
-      pose proof (mem_out_some Monoid_RthetaSafeFlags  (svector_to_mem_block x) ) as M.
-      apply is_Some_equiv_def in M.
-      destruct M as [y M].
-      rewrite M.
-      f_equiv.
-      unfold equiv, mem_block_Equiv, mem_block_equiv, NM.Equal.
-      intros k.
-
-      unfold svector_to_mem_block in *.
-      svector_to_mem_block_to_spec m0 H0 I0 O0.
-      svector_to_mem_block_to_spec m1 H1 I1 O1.
-      simpl in *.
-
-      unfold mem_op_of_hop in M.
-      break_match_hyp; try some_none.
-      some_inv.
-      rewrite <- M. clear M.
-
-      unfold avector_to_mem_block.
-      avector_to_mem_block_to_spec m2 H2 O2.
-      unfold mem_lookup in *. simpl in *.
-
-      destruct (NatUtil.lt_ge_dec k o) as [kc | kc].
-      +
-        (* k<n, which is normal *)
-        clear O0 O1 O2.
-        specialize (H0 k kc). specialize (I0 k kc).
-        assert (k < o + o)%nat as kc1 by omega.
-        assert(V1: Is_Val (Vnth x kc1)).
-        {
-          apply G.
-          apply Full_intro.
-        }
-
-        assert (k + o < o + o)%nat as kc2 by omega.
-        assert(V2: Is_Val (Vnth x kc2)).
-        {
-          apply G.
-          apply Full_intro.
-        }
-
-        assert(V: Is_Val (Vnth (SHBinOp' f x) kc)).
-        {
-          erewrite SHBinOp'_nth with (jc:=kc).
-          apply Is_Val_Safe_liftM2.
-          apply V1.
-          apply V2.
-        }
-
-        rewrite H0 in V.
-        apply NM.find_1 in V.
-        rewrite V.
-
-        rewrite H2 with (ip:=kc).
+        assert((∀ (j : nat) (jc : j < o+o), in_index_set Monoid_RthetaSafeFlags
+                                                       (SHBinOp Monoid_RthetaSafeFlags f)
+                                                       (mkFinNat jc) →
+                                          mem_in j (svector_to_mem_block x))
+               → is_Some (mem_op_of_hop (HBinOp f) (svector_to_mem_block x))) as M by apply mem_out_some_mem_op_of_hop.
+        apply is_Some_equiv_def in M.
+        destruct M as [y M].
+        rewrite M.
         f_equiv.
-        rewrite SHBinOp'_nth with (jc:=kc) (jc1:=kc1) (jc2:=kc2).
-        rewrite HBinOp_nth with (jc:=kc) (jc1:=kc1) (jc2:=kc2).
+        unfold equiv, mem_block_Equiv, mem_block_equiv, NM.Equal.
+        intros k.
 
-        rewrite evalWriter_Rtheta_liftM2.
-        f_equiv.
-        *
-          specialize (H1 k kc1).
-          unfold mem_block_to_avector in Heqo0.
-          apply vsequence_Vbuild_eq_Some in Heqo0.
-          apply Vnth_arg_eq with (ip:=kc1) in Heqo0.
-          rewrite Vbuild_nth in Heqo0.
-          rewrite Vnth_map in Heqo0.
-          unfold mem_lookup in Heqo0.
+        unfold svector_to_mem_block in *.
+        svector_to_mem_block_to_spec m0 H0 I0 O0.
+        svector_to_mem_block_to_spec m1 H1 I1 O1.
+        simpl in *.
 
-          apply H1 in V1.
-          apply NM.find_1 in V1.
-          rewrite Heqo0 in V1.
-          some_inv.
+        unfold mem_op_of_hop in M.
+        break_match_hyp; try some_none.
+        some_inv.
+        rewrite <- M. clear M.
+
+        unfold avector_to_mem_block.
+        avector_to_mem_block_to_spec m2 H2 O2.
+        unfold mem_lookup in *. simpl in *.
+
+        destruct (NatUtil.lt_ge_dec k o) as [kc | kc].
+        +
+          (* k<n, which is normal *)
+          clear O0 O1 O2.
+          specialize (H0 k kc). specialize (I0 k kc).
+          assert (k < o + o)%nat as kc1 by omega.
+          assert(V1: Is_Val (Vnth x kc1)).
+          {
+            apply G.
+            apply Full_intro.
+          }
+
+          assert (k + o < o + o)%nat as kc2 by omega.
+          assert(V2: Is_Val (Vnth x kc2)).
+          {
+            apply G.
+            apply Full_intro.
+          }
+
+          assert(V: Is_Val (Vnth (SHBinOp' f x) kc)).
+          {
+            erewrite SHBinOp'_nth with (jc:=kc).
+            apply Is_Val_Safe_liftM2.
+            apply V1.
+            apply V2.
+          }
+
+          rewrite H0 in V.
+          apply NM.find_1 in V.
+          rewrite V.
+
+          rewrite H2 with (ip:=kc).
+          f_equiv.
+          rewrite SHBinOp'_nth with (jc:=kc) (jc1:=kc1) (jc2:=kc2).
+          rewrite HBinOp_nth with (jc:=kc) (jc1:=kc1) (jc2:=kc2).
+
+          rewrite evalWriter_Rtheta_liftM2.
+          f_equiv.
+          *
+            specialize (H1 k kc1).
+            unfold mem_block_to_avector in Heqo0.
+            apply vsequence_Vbuild_eq_Some in Heqo0.
+            apply Vnth_arg_eq with (ip:=kc1) in Heqo0.
+            rewrite Vbuild_nth in Heqo0.
+            rewrite Vnth_map in Heqo0.
+            unfold mem_lookup in Heqo0.
+
+            apply H1 in V1.
+            apply NM.find_1 in V1.
+            rewrite Heqo0 in V1.
+            some_inv.
+            reflexivity.
+          *
+            specialize (H1 (k+o)%nat kc2).
+            unfold mem_block_to_avector in Heqo0.
+            apply vsequence_Vbuild_eq_Some in Heqo0.
+            apply Vnth_arg_eq with (ip:=kc2) in Heqo0.
+            rewrite Vbuild_nth in Heqo0.
+            rewrite Vnth_map in Heqo0.
+            unfold mem_lookup in Heqo0.
+
+            apply H1 in V2.
+            apply NM.find_1 in V2.
+            rewrite Heqo0 in V2.
+            some_inv.
+            reflexivity.
+        +
+          rewrite O0 by apply kc.
+          rewrite O2 by apply kc.
           reflexivity.
-        *
-          specialize (H1 (k+o)%nat kc2).
-          unfold mem_block_to_avector in Heqo0.
-          apply vsequence_Vbuild_eq_Some in Heqo0.
-          apply Vnth_arg_eq with (ip:=kc2) in Heqo0.
-          rewrite Vbuild_nth in Heqo0.
-          rewrite Vnth_map in Heqo0.
-          unfold mem_lookup in Heqo0.
-
-          apply H1 in V2.
-          apply NM.find_1 in V2.
-          rewrite Heqo0 in V2.
-          some_inv.
-          reflexivity.
-      +
-        rewrite O0 by apply kc.
-        rewrite O2 by apply kc.
-        reflexivity.
-      +
-        intros j jc HH.
-        apply svector_to_mem_block_In with (jc0:=jc).
-        apply G,HH.
+        +
+          intros j jc HH.
+          apply svector_to_mem_block_In with (jc0:=jc).
+          apply G,HH.
     Qed.
 
     (* TODO: move to memory. add similar to m2. *)
@@ -700,8 +1227,53 @@ Section MemVecEq.
         apply Intersection_intro; auto.
     Qed.
 
+    Fact HTSUMUnion_mem_out_fill_pattern
+         {i o : nat}
+         {dot : SgOp CarrierA}
+         {dot_mor : Proper (equiv ==> equiv ==> equiv) dot}
+         (op1 op2 : SHOperator Monoid_RthetaFlags)
+         `{Meq1: SHOperator_Mem _ i o op1}
+         `{Meq2: SHOperator_Mem _ i o op2} :
+      forall (m0 m : mem_block),
+        HTSUMUnion_mem (mem_op (xop:=op1)) (mem_op (xop:=op2)) m0 ≡ Some m
+        → forall (j : nat) (jc : j < o),
+          out_index_set (i:=i) Monoid_RthetaFlags
+                        (HTSUMUnion Monoid_RthetaFlags dot op1
+                                    op2) (mkFinNat jc) ↔
+                        mem_in j m.
+    Proof.
+      intros m0 m E.
+      split; intros H.
+      +
+        simpl in *.
+        unfold HTSUMUnion_mem in E.
+        repeat break_match_hyp; try some_none.
+        apply mem_merge_key_dec with (m0:=m1) (m1:=m2) (k:=j) in E.
+        destruct E as [E0 E1].
+        dependent destruction H; apply E1.
+        *
+          left.
+          eapply (out_mem_fill_pattern _ _ Heqo0); eauto.
+        *
+          right.
+          eapply (out_mem_fill_pattern _ _ Heqo1); eauto.
+      +
+        simpl in *.
+        unfold HTSUMUnion_mem in E.
+        repeat break_match_hyp; try some_none.
+        apply mem_merge_key_dec with (m0:=m1) (m1:=m2) (k:=j) in E.
+        destruct E as [E0 E1].
+        specialize (E0 H). clear H E1.
+        destruct E0 as [M1 | M2].
+        *
+          apply Union_introl.
+          eapply (out_mem_fill_pattern _ _ Heqo0); eauto.
+        *
+          right.
+          eapply (out_mem_fill_pattern _ _ Heqo1); eauto.
+    Qed.
 
-    Global Instance HTSUMUnion_MemVecEq
+    Global Instance HTSUMUnion_Mem
            {i o: nat}
            `{dot: SgOp CarrierA}
            `{dot_mor: !Proper ((=) ==> (=) ==> (=)) dot}
@@ -710,8 +1282,8 @@ Section MemVecEq.
                              (out_index_set _ op1)
                              (out_index_set _ op2)
            )
-           `{Meq1: SHOperator_MemVecEq _ i o op1}
-           `{Meq2: SHOperator_MemVecEq _ i o op2}
+           `{Meq1: SHOperator_Mem _ i o op1}
+           `{Meq2: SHOperator_Mem _ i o op2}
 
            `{a_zero: MonUnit CarrierA}
            (* `a_zero` together with `dot` form a monoid. NONE: using `eq` here *)
@@ -727,257 +1299,339 @@ Section MemVecEq.
                ¬ out_index_set _ op2 (mkFinNat tc) ->
                evalWriter (Vnth (op Monoid_RthetaFlags op2 x) tc) ≡ a_zero)
 
-      : SHOperator_MemVecEq
+      : SHOperator_Mem
           (facts := HTSUMUnion_Facts dot op1 op2 compat)
           (HTSUMUnion Monoid_RthetaFlags dot op1 op2).
     Proof.
-      split.
-      intros x G.
-      simpl.
-      unfold HTSUMUnion', Vec2Union, HTSUMUnion_mem.
-      break_match.
+      unshelve esplit.
       -
+        apply (HTSUMUnion_mem
+                 (mem_op (xop:=op1))
+                 (mem_op (xop:=op2))).
+      -
+        apply HTSUMUnion_mem_proper; [apply Meq1 | apply Meq2].
+      -
+        (* mem_out_some *)
+        intros m H.
+        unfold is_Some, HTSUMUnion, HTSUMUnion_mem in *.
+        simpl in *.
+        repeat break_match; try some_none; try auto.
+        +
+          contradict Heqo0.
+          clear H.
+          apply mem_merge_is_Some.
+          pose proof (out_mem_fill_pattern m m0 Heqo1) as P1.
+          pose proof (out_mem_oob m m0 Heqo1) as NP1.
+          pose proof (out_mem_fill_pattern m m1 Heqo2) as P2.
+          pose proof (out_mem_oob m m1 Heqo2) as NP2.
+
+          apply Disjoint_intro.
+          intros j.
+          destruct (NatUtil.lt_ge_dec j o) as [jc | jc].
+          *
+            clear NP1 NP2.
+            specialize (P1 j jc).
+            specialize (P2 j jc).
+            destruct compat as [compat].
+            specialize (compat (mkFinNat jc)).
+            intros C.
+            unfold In, not  in *.
+            destruct C as [j H0 H1].
+
+            apply NE.In_In, mem_keys_set_In, P1 in H0. clear P1.
+            apply NE.In_In, mem_keys_set_In, P2 in H1. clear P2.
+            destruct compat.
+            apply Intersection_intro; auto.
+          *
+            specialize (NP1 j jc).
+            intros C.
+            destruct C as [j H0 _].
+            apply NE.In_In, mem_keys_set_In in H0.
+            unfold mem_in in NP1.
+            congruence.
+        +
+          clear Heqo0.
+          contradict Heqo2.
+          apply is_Some_ne_None.
+          apply mem_out_some; auto.
+          intros j jc H0.
+          specialize (H j jc).
+          apply H.
+          apply Union_intror.
+          apply H0.
+        +
+          clear Heqo0.
+          contradict Heqo1.
+          apply is_Some_ne_None.
+          apply mem_out_some; auto.
+          intros j jc H0.
+          specialize (H j jc).
+          apply H.
+          apply Union_introl.
+          apply H0.
+      -
+        (* out_mem_fill_pattern *)
+        apply HTSUMUnion_mem_out_fill_pattern.
+      -
+        intros m0 m E j jc H.
+        simpl in *.
+        unfold HTSUMUnion_mem in E.
+        repeat break_match_hyp; try some_none.
+        apply mem_merge_key_dec with (m0:=m1) (m1:=m2) (k:=j) in E.
+        destruct E as [E0 E1].
+        specialize (E0 H). clear H E1.
+        destruct E0 as [M0 | M1].
+        --
+          eapply (out_mem_oob _ _ Heqo0); eauto.
+        --
+          eapply (out_mem_oob _ _ Heqo1); eauto.
+      -
+        intros x G.
+        simpl.
+        unfold HTSUMUnion', Vec2Union, HTSUMUnion_mem.
         break_match.
         +
-          (* both mem_ops return Some *)
-          rename m into m1, m0 into m2. (* to match operator indices *)
-          destruct (mem_merge m1 m2) eqn:MM.
+          break_match.
           *
-            apply RelUtil.opt_r_Some.
-            unfold mem_block_Equiv, mem_block_equiv, NM.Equal.
-            intros k.
-            unfold svector_to_mem_block.
-            svector_to_mem_block_to_spec m' H0 H1 I2.
-            simpl in *.
-            destruct (NatUtil.lt_ge_dec k o) as [kc | kc].
+            (* both mem_ops return Some *)
+            rename m into m1, m0 into m2. (* to match operator indices *)
+            destruct (mem_merge m1 m2) eqn:MM.
             --
-              clear I2.
-              (* k<o. Normal *)
-              (* each k could be either in out_set of op1 or op2 *)
-              specialize (H0 k kc).
-              specialize (H1 k kc).
-
-              rename facts0 into facts2,  facts into facts1.
-              pose proof (out_mem_fill_pattern _
-                                               (SHOperator_Facts:=HTSUMUnion_Facts dot op1 op2 compat)
-                         ) as P.
-              specialize (P (svector_to_mem_block x) m).
-              simpl in P.
-              unfold HTSUMUnion_mem in P.
-              break_match_hyp; try some_none.
-              break_match_hyp; try some_none.
-              some_inv; subst m3.
-              some_inv; subst m0.
-              specialize (P MM).
-              destruct P as [P _].
-              specialize (P k kc).
-              destruct (NP.F.In_dec m k) as [K | NK].
+              apply RelUtil.opt_r_Some.
+              unfold mem_block_Equiv, mem_block_equiv, NM.Equal.
+              intros k.
+              unfold svector_to_mem_block.
+              svector_to_mem_block_to_spec m' H0 H1 I2.
+              simpl in *.
+              destruct (NatUtil.lt_ge_dec k o) as [kc | kc].
               ++
-                (* k in m *)
-                pose proof (mem_merge_key_dec m m1 m2 MM k) as [MD _].
-                specialize (MD K).
-                clear H1.
-                apply P in K; clear P.
-                pose proof (out_as_range _ x (SHOperator_Facts:=HTSUMUnion_Facts dot op1 op2 compat) G k kc) as V.
-                apply V in K; clear V.
-                assert(V:=K).
-                apply H0 in K; clear H0.
-                apply NM.find_1 in K.
-                rewrite_clear K.
-                rewrite Vnth_map2.
+                clear I2.
+                (* k<o. Normal *)
+                (* each k could be either in out_set of op1 or op2 *)
+                specialize (H0 k kc).
+                specialize (H1 k kc).
 
-                simpl in V.
-                unfold mem_merge in MM.
-                break_if; try some_none.
-                some_inv.
-                subst m.
-                unfold mem_union.
-                rewrite NM.map2_1 by (destruct MD; auto).
+                rename facts0 into facts2,  facts into facts1.
 
-                inversion MD.
+                pose proof (HTSUMUnion_mem_out_fill_pattern op1 op2 ) as P.
+                specialize (P (svector_to_mem_block x) m).
+                simpl in P.
+                unfold HTSUMUnion_mem in P.
+                break_match_hyp; try some_none.
+                break_match_hyp; try some_none.
+                some_inv; subst m3.
+                some_inv; subst m0.
+                specialize (P MM).
+                specialize (P k kc).
+                destruct (NP.F.In_dec m k) as [K | NK].
                 **
-                  (* k in m1 *)
-                  rename H into M1.
-                  assert(NM2: not (NM.In (elt:=CarrierA) k m2)).
-                  {
-                    apply mem_keys_disjoint_inr with (m1:=m1).
-                    apply Heqb.
-                    apply M1.
-                  }
-                  break_match; try (apply NP.F.not_find_in_iff in Heqo0; congruence).
+                  (* k in m *)
+                  pose proof (mem_merge_key_dec m m1 m2 MM k) as [MD _].
+                  specialize (MD K).
+                  clear H1.
+                  apply P in K; clear P.
+                  pose proof (out_as_range _ x (SHOperator_Facts:=HTSUMUnion_Facts dot op1 op2 compat) G k kc) as V.
+                  apply V in K; clear V.
+                  assert(V:=K).
+                  apply H0 in K; clear H0.
+                  apply NM.find_1 in K.
+                  rewrite_clear K.
+                  rewrite Vnth_map2.
 
-
-                  (* derive m1[k] *)
-                  assert (G1: (∀ (j : nat) (jc : (j < i)%nat), in_index_set Monoid_RthetaFlags op1 (mkFinNat jc) →  Is_Val (Vnth x jc))).
-                  {
-                    intros j jc H.
-                    apply G.
-                    apply Union_introl.
-                    apply H.
-                  }
-                  apply Meq1 in G1; clear Meq1.
-                  rewrite Heqo2 in G1.
+                  simpl in V.
+                  unfold mem_merge in MM.
+                  break_if; try some_none.
                   some_inv.
-                  unfold equiv, mem_block_Equiv, mem_block_equiv, NM.Equal in G1.
-                  rewrite <- Heqo0.
-                  rewrite <- G1.
+                  subst m.
+                  unfold mem_union.
+                  rewrite NM.map2_1 by (destruct MD; auto).
 
-                  rewrite find_svector_to_mem_block_some with (kc:=kc).
-                  2:{
-                    apply NP.F.in_find_iff.
-                    rewrite G1.
-                    apply NP.F.in_find_iff.
-                    apply M1.
-                  }
+                  inversion MD.
+                  ---
+                    (* k in m1 *)
+                    rename H into M1.
+                    assert(NM2: not (NM.In (elt:=CarrierA) k m2)).
+                    {
+                      apply mem_keys_disjoint_inr with (m1:=m1).
+                      apply Heqb.
+                      apply M1.
+                    }
+                    break_match; try (apply NP.F.not_find_in_iff in Heqo0; congruence).
 
-                  f_equiv.
-                  unfold SVector.Union.
-                  rewrite evalWriter_Rtheta_liftM2.
 
-                  pose proof (out_mem_fill_pattern Monoid_RthetaFlags (svector_to_mem_block x) m2 Heqo3) as [P2 _].
-                  unfold mem_in in P2. specialize (P2 k kc).
-                  apply not_iff_compat in P2.
-                  apply P2 in NM2.
-                  apply Z2 with (x:=x) in NM2.
-                  rewrite NM2.
-                  apply monoid_right_id.
-                  apply af_mon.
+                    (* derive m1[k] *)
+                    assert (G1: (∀ (j : nat) (jc : (j < i)%nat), in_index_set Monoid_RthetaFlags op1 (mkFinNat jc) →  Is_Val (Vnth x jc))).
+                    {
+                      intros j jc H.
+                      apply G.
+                      apply Union_introl.
+                      apply H.
+                    }
+                    apply Meq1 in G1.
+                    rewrite Heqo2 in G1.
+                    some_inv.
+                    unfold equiv, mem_block_Equiv, mem_block_equiv, NM.Equal in G1.
+                    rewrite <- Heqo0.
+                    rewrite <- G1.
+
+                    rewrite find_svector_to_mem_block_some with (kc:=kc).
+                    2:{
+                      apply NP.F.in_find_iff.
+                      rewrite G1.
+                      apply NP.F.in_find_iff.
+                      apply M1.
+                    }
+
+                    f_equiv.
+                    unfold SVector.Union.
+                    rewrite evalWriter_Rtheta_liftM2.
+
+                    pose proof (out_mem_fill_pattern _ _ Heqo3) as P2.
+                    unfold mem_in in P2. specialize (P2 k kc).
+                    apply not_iff_compat in P2.
+                    apply P2 in NM2.
+                    apply Z2 with (x:=x) in NM2.
+                    rewrite NM2.
+                    apply monoid_right_id.
+                    apply af_mon.
+                  ---
+                    (* k in m2 *)
+                    rename H into M2.
+                    assert(NM1: not (NM.In (elt:=CarrierA) k m1)).
+                    {
+                      apply mem_keys_disjoint_inr with (m1:=m2).
+                      rewrite is_disjoint_sym.
+                      apply Heqb.
+                      apply M2.
+                    }
+                    break_match; try (apply NP.F.not_find_in_iff in NM1; congruence).
+                    clear Heqo0.
+
+                    (* derive m2[k] *)
+                    assert (G2: (∀ (j : nat) (jc : (j < i)%nat), in_index_set Monoid_RthetaFlags op2 (mkFinNat jc) →  Is_Val (Vnth x jc))).
+                    {
+                      intros j jc H.
+                      apply G.
+                      apply Union_intror.
+                      apply H.
+                    }
+                    apply Meq2 in G2.
+                    rewrite Heqo3 in G2.
+                    some_inv.
+                    unfold equiv, mem_block_Equiv, mem_block_equiv, NM.Equal in G2.
+                    rewrite <- G2.
+
+                    rewrite find_svector_to_mem_block_some with (kc:=kc).
+                    2:{
+                      apply NP.F.in_find_iff.
+                      rewrite G2.
+                      apply NP.F.in_find_iff.
+                      apply M2.
+                    }
+
+                    f_equiv.
+                    unfold SVector.Union.
+                    rewrite evalWriter_Rtheta_liftM2.
+
+                    pose proof (out_mem_fill_pattern _ _ Heqo2) as P1.
+                    unfold mem_in in P1. specialize (P1 k kc).
+                    apply not_iff_compat in P1.
+                    apply P1 in NM1.
+                    apply Z1 with (x:=x) in NM1 .
+                    rewrite NM1.
+                    apply monoid_left_id.
+                    apply af_mon.
                 **
-                  (* k in m2 *)
-                  rename H into M2.
-                  assert(NM1: not (NM.In (elt:=CarrierA) k m1)).
-                  {
-                    apply mem_keys_disjoint_inr with (m1:=m2).
-                    rewrite is_disjoint_sym.
-                    apply Heqb.
-                    apply M2.
-                  }
-                  break_match; try (apply NP.F.not_find_in_iff in NM1; congruence).
-                  clear Heqo0.
-
-                  (* derive m2[k] *)
-                  assert (G2: (∀ (j : nat) (jc : (j < i)%nat), in_index_set Monoid_RthetaFlags op2 (mkFinNat jc) →  Is_Val (Vnth x jc))).
-                  {
-                    intros j jc H.
-                    apply G.
-                    apply Union_intror.
-                    apply H.
-                  }
-                  apply Meq2 in G2; clear Meq2.
-                  rewrite Heqo3 in G2.
-                  some_inv.
-                  unfold equiv, mem_block_Equiv, mem_block_equiv, NM.Equal in G2.
-                  rewrite <- G2.
-
-                  rewrite find_svector_to_mem_block_some with (kc:=kc).
-                  2:{
-                    apply NP.F.in_find_iff.
-                    rewrite G2.
-                    apply NP.F.in_find_iff.
-                    apply M2.
-                  }
-
-                  f_equiv.
-                  unfold SVector.Union.
-                  rewrite evalWriter_Rtheta_liftM2.
-
-                  pose proof (out_mem_fill_pattern Monoid_RthetaFlags (svector_to_mem_block x) m1 Heqo2) as [P1 _].
-                  unfold mem_in in P1. specialize (P1 k kc).
-                  apply not_iff_compat in P1.
-                  apply P1 in NM1.
-                  apply Z1 with (x:=x) in NM1 .
-                  rewrite NM1.
-                  apply monoid_left_id.
-                  apply af_mon.
+                  (* k not in m *)
+                  replace (NM.find (elt:=CarrierA) k m) with (@None CarrierA)
+                    by (symmetry; apply NP.F.not_find_in_iff, NK).
+                  apply not_iff_compat in P.
+                  apply P in NK; clear P.
+                  pose proof (no_vals_at_sparse _ x k kc (SHOperator_Facts:=HTSUMUnion_Facts dot op1 op2 compat)) as NV.
+                  apply NV in NK; clear NV.
+                  apply not_Is_Val_Is_Struct in NK.
+                  apply not_iff_compat in H1.
+                  apply H1 in NK; clear H1.
+                  apply NP.F.not_find_in_iff in NK.
+                  rewrite NK.
+                  reflexivity.
               ++
-                (* k not in m *)
-                replace (NM.find (elt:=CarrierA) k m) with (@None CarrierA)
-                  by (symmetry; apply NP.F.not_find_in_iff, NK).
-                apply not_iff_compat in P.
-                apply P in NK; clear P.
-                pose proof (no_vals_at_sparse _ x k kc (SHOperator_Facts:=HTSUMUnion_Facts dot op1 op2 compat)) as NV.
-                apply NV in NK; clear NV.
-                apply not_Is_Val_Is_Struct in NK.
-                apply not_iff_compat in H1.
-                apply H1 in NK; clear H1.
-                apply NP.F.not_find_in_iff in NK.
-                rewrite NK.
-                reflexivity.
+                (* k>=o. m[k] should be None *)
+                clear H0 H1.
+                specialize (I2 k kc).
+                unfold mem_lookup in I2.
+                rewrite_clear I2.
+                symmetry.
+                apply NP.F.not_find_in_iff.
+                intros N.
+                apply (mem_merge_key_dec m m1 m2 MM k) in N.
+                generalize dependent (svector_to_mem_block x).
+                intros m0 H1 H2.
+                destruct N as [IN1 | IN2].
+                **
+                  (* prove contradiction in N1 *)
+                  pose proof (out_mem_oob _ _ H1) as NP1.
+                  specialize (NP1 k kc).
+                  unfold mem_in in NP1.
+                  congruence.
+                **
+                  (* prove contradiction in N1 *)
+                  pose proof (out_mem_oob _ _ H2) as NP2.
+                  specialize (NP2 k kc).
+                  unfold mem_in in NP2.
+                  congruence.
             --
-              (* k>=o. m[k] should be None *)
-              clear H0 H1.
-              specialize (I2 k kc).
-              unfold mem_lookup in I2.
-              rewrite_clear I2.
-              symmetry.
-              apply NP.F.not_find_in_iff.
-              intros N.
-              apply (mem_merge_key_dec m m1 m2 MM k) in N.
+              contradict MM.
+              apply mem_merge_is_Some.
+              apply Disjoint_intro.
+              intros k.
+              intros H.
+              unfold Ensembles.In in H.
+              destruct H.
+              rename x0 into k.
+              rename H into IN1, H0 into IN2.
+              apply NE.In_In, mem_keys_set_In in IN1.
+              apply NE.In_In,mem_keys_set_In in IN2.
               generalize dependent (svector_to_mem_block x).
-              intros m0 H1 H2.
-              destruct N as [IN1 | IN2].
+              intros m H1 H2.
+              (* by `compat` hypothes, output index sets of op1 and op2 are disjoint.
+               yet, but IN1 and IN2, 'k' belongs to both *)
+              pose proof (out_mem_fill_pattern _ _ H1) as P1.
+              pose proof (out_mem_oob _ _ H1) as NP1.
+              pose proof (out_mem_fill_pattern _ _ H2) as P2.
+              pose proof (out_mem_oob _ _ H2) as NP2.
+              destruct (NatUtil.lt_ge_dec k o) as [kc | nkc].
               ++
-                (* prove contradiction in N1 *)
-                pose proof (out_mem_fill_pattern Monoid_RthetaFlags m0 m1 H1) as [P1 NP1].
-                specialize (NP1 k kc).
+                clear NP1 NP2.
+                apply (P1 k kc) in IN1; clear P1.
+                apply (P2 k kc) in IN2; clear P2.
+                inversion_clear compat.
+                specialize (H (mkFinNat kc)).
+                crush.
+              ++
+                specialize (NP1 k nkc).
                 unfold mem_in in NP1.
                 congruence.
-              ++
-                (* prove contradiction in N1 *)
-                pose proof (out_mem_fill_pattern Monoid_RthetaFlags m0 m2 H2) as [P2 NP2].
-                specialize (NP2 k kc).
-                unfold mem_in in NP2.
-                congruence.
           *
-            contradict MM.
-            apply mem_merge_is_Some.
-            apply Disjoint_intro.
-            intros k.
-            intros H.
-            unfold In in H.
-            destruct H.
-            rename x0 into k.
-            rename H into IN1, H0 into IN2.
-            apply NE.In_In, mem_keys_set_In in IN1.
-            apply NE.In_In,mem_keys_set_In in IN2.
-            generalize dependent (svector_to_mem_block x).
-            intros m H1 H2.
-            (* by `compat` hypothes, output index sets of op1 and op2 are disjoint.
-               yet, but IN1 and IN2, 'k' belongs to both *)
-            pose proof (out_mem_fill_pattern Monoid_RthetaFlags m m1 H1) as [P1 NP1].
-            pose proof (out_mem_fill_pattern Monoid_RthetaFlags m m2 H2) as [P2 NP2].
-            destruct (NatUtil.lt_ge_dec k o) as [kc | nkc].
-            --
-              clear NP1 NP2.
-              apply (P1 k kc) in IN1; clear P1.
-              apply (P2 k kc) in IN2; clear P2.
-              inversion_clear compat.
-              specialize (H (mkFinNat kc)).
-              crush.
-            --
-              specialize (NP1 k nkc).
-              unfold mem_in in NP1.
-              congruence.
+            contradict Heqo1.
+            apply is_Some_ne_None.
+            apply mem_out_some; auto.
+            intros j jc H.
+            apply svector_to_mem_block_In with (jc0:=jc).
+            apply G.
+            simpl.
+            apply Union_intror.
+            apply H.
         +
-          contradict Heqo1.
+          contradict Heqo0.
           apply is_Some_ne_None.
           apply mem_out_some; auto.
           intros j jc H.
           apply svector_to_mem_block_In with (jc0:=jc).
           apply G.
           simpl.
-          apply Union_intror.
+          apply Union_introl.
           apply H.
-      -
-        contradict Heqo0.
-        apply is_Some_ne_None.
-        apply mem_out_some; auto.
-        intros j jc H.
-        apply svector_to_mem_block_In with (jc0:=jc).
-        apply G.
-        simpl.
-        apply Union_introl.
-        apply H.
     Qed.
 
   End MonoidSpecific.
